$$ (a + b) \text{ mod } m = (a \text{ mod } m + b \text{ mod } m) \text{ mod } m $$
$$ (a - b) \text{ mod } m = (a \text{ mod } m - b \text{ mod } m) \text{ mod } m $$
$$ (a \times b) \text{ mod } m = ((a \text{ mod } m) \times (b \text{ mod } m)) \text{ mod } m $$
$$ a^b \text{ mod } m = (a \text{ mod } m)^b \text{ mod } m $$
$$ a \equiv b \text{ } (\text{mod } m) \iff (b - a) \vert m $$

$$ \gcd(a_1, a_2, a_3, a_4) = \gcd(a_1, \gcd(a_2, \gcd(a_3, a_4))) $$
$$ \lcm(a, b) \times \gcd(a, b) = a \times b $$
$$ \lcm(a, b) = \dfrac{a \times b}{\gcd(a, b)} = \dfrac{a}{\gcd(a,b)} \times b $$