\subsection{Logarithm}

$$ \log _{b} mn = \log _{b} m + \log _{b} n \quad\quad log _{b} \dfrac{m}{n} = \log _{b} m - \log _{n} n \quad\quad \log _{b} n^p = p \log _{b} n$$
$$ \log _{b} \sqrt[q]{n} = \dfrac{1}{q} \log _{b} n \quad\quad \log _{b} n = \log _{a} n \log _{b} a \quad\quad b^{\log _{b} k} = k $$
$$ \log _{b} a = \dfrac{\log _{c} a}{\log _{c} b} \quad\quad \log _{b} a = \dfrac{1}{\log _{a} b} \quad\quad \log _{b} a \text{ } \log _{a} c = \log _{b} c $$
$$ \log _{b} 1 = 0 \quad\quad \log _{b} b = 1 $$
